new upstream version of RelationAlgebra: 1.1
git-svn-id: svn://scm.gforge.inria.fr/svnroot/coq-contribs/trunk@2221 0cf17b13-060f-0410-b1b1-c666bec9822a

imp.v
@@ -1,10 +1,10 @@
-(*******************************************************************)
-(*  This is part of RelationAlgebra, it is distributed under the   *)
-(*    terms of the GNU Lesser General Public License version 3     *)
-(*              (see file LICENSE for more details)                *)
-(*                                                                 *)
-(*  Copyright 2012: Damien Pous. (CNRS, LIP - ENS Lyon, UMR 5668)  *)
-(*******************************************************************)
+(************************************************************************)
+(*    This is part of RelationAlgebra, it is distributed under the      *)
+(*      terms of the GNU Lesser General Public License version 3        *)
+(*                (see file LICENSE for more details)                   *)
+(*                                                                      *)
+(*  Copyright 2012-2013: Damien Pous. (CNRS, LIP - ENS Lyon, UMR 5668)  *)
+(************************************************************************)
 
 (** * imp: a formalisation of the IMP programming language on top of KAT *)
 
@@ -18,117 +18,39 @@
    for partial correctness. *)
 
 Require Import kat prop rel comparisons kat_tac.
-Require Import String FunctionalExtensionality.
-Open Scope string_scope.
+
+Section s.
+(** identifiers for memory locations  *)
+Variable loc: Set.
+(** abstract state (or memory) *)
+Variable state: Set.
+(** updating the state *)
+Variable update: loc -> nat -> state -> state.
 
 (** * Definition of the languague *)
 
-(** we use string to denote locations (variables) *)
-
-Definition string_compare x y := if string_dec x y then Eq else Lt.
-Lemma string_cmp_spec: forall x y, compare_spec (x=y) (string_compare x y).
-Proof. intros. unfold string_compare. case string_dec; constructor; congruence. Qed.
-Canonical Structure string_cmp := mk_simple_cmp _ string_cmp_spec.
-
-
-(** state (or memory): a map from strings (locations) to natural numbers *)
-
-Definition state := string -> nat.
-
-
-(** ** arithmetic expressions *)
-
-Inductive expr :=
-| var (x: string)
-| cst (k: nat)
-| pls (e f: expr)
-| min (e f: expr)
-| mul (e f: expr).
-
-(** coercions and notations  *)
-Coercion var: string >-> expr.
-Coercion cst: nat >-> expr.
-Bind Scope e_scope with expr.
-Delimit Scope e_scope with e.
-Infix "+" := pls: e_scope.
-Infix "-" := min: e_scope.
-Infix "*" := mul: e_scope.
-Notation "0" := O: e_scope.
-Notation "1" := (S O): e_scope.
-Arguments pls _%e _%e. 
-Arguments min _%e _%e. 
-Arguments mul _%e _%e. 
-
-(** evaluation of arithmetic expressions *)
-Fixpoint eval e (s: state) :=
-  match e with
-    | var x => s x
-    | cst k => k
-    | pls e f => eval e s + eval f s
-    | mul e f => eval e s * eval f s
-    | min e f => eval e s - eval f s
-  end%nat.
-
-(** ** Boolean tests *)
-
-Inductive test :=
-| tst (e f: expr)
-| cnj (e f: test)
-| dsj (e f: test)
-| neg (f: test)
-| top
-| bot.
-
-(** notations *)
-Bind Scope t_scope with test.
-Delimit Scope t_scope with t.
-Infix "?=" := tst (at level 80): t_scope.
-Infix "&&" := cnj: t_scope.
-Infix "||" := dsj: t_scope.
-Arguments cnj _%t _%t.
-Arguments dsj _%t _%t.
-Arguments neg _%t.
-
-(** evaluation of Boolean tests *)
-Fixpoint teval e: dset state :=
-  match e with
-    | tst e f => fun s => eqb (eval e s) (eval f s)
-    | cnj e f => teval e \cap teval f
-    | dsj e f => teval e \cup teval f
-    | neg e => ! teval e
-    | top => lattice.top
-    | bot => lattice.bot
-  end.
-Coercion teval: test >-> car.
-
-
-
-(** ** programs *)
+(** programs *)
 
 Inductive prog :=
 | skp
-| aff (x: string) (e: expr)
+| aff (x: loc) (e: state -> nat)
 | seq (p q: prog)
-| ite (t: test) (p q: prog)
-| whl (t: test) (p: prog).
+| ite (t: dset state) (p q: prog)
+| whl (t: dset state) (p: prog).
 
 (** notations *)
 Bind Scope imp_scope with prog.
 Delimit Scope imp_scope with imp.
-Notation "x  <- y" := (aff x%string y%e) (at level 90): imp_scope.
+Notation "x  <- y" := (aff x y) (at level 90): imp_scope.
 Notation "p  ;; q" := (seq p%imp q%imp) (left associativity, at level 101): imp_scope.
-Arguments ite _%t _%imp _%imp.
-Arguments whl _%t _%imp.
+Arguments ite _%ra _%imp _%imp.
+Arguments whl _%ra _%imp.
 
 
 (** * Big step semantics *)
 
-(** updating a state, by assigning a new value [i] to [x] *)
-Definition update x i (s: state): state :=
-  fun y => if eqb x y then i else s y.
-
 (** corresponding functional relation *)
-Notation upd x e := (frel (fun s => update x (eval e s) s)).
+Notation upd x e := (frel (fun s => update x (e s) s)).
 
 
 (** ** using KAT expressions in the model of relations
@@ -141,20 +63,20 @@ Fixpoint bstep (p: prog): rel state state :=
     | skp => 1
     | aff x e => upd x e
     | seq p q => bstep p * bstep q
-    | ite t p q => [t] * bstep p + [!t] * bstep q
-    | whl t p => ([t] * bstep p)^*  *  [!t]
+    | ite b p q => [b] * bstep p + [!b] * bstep q
+    | whl b p => ([b] * bstep p)^*  *  [!b]
   end.
 
 (** ** using an inductive predicate, as in standard textbooks *)
 
 Inductive bstep': prog -> rel state state :=
 | s_skp: forall s, bstep' skp s s
-| s_aff: forall x e s, bstep' (x <- e) s (update x (eval e s) s)
+| s_aff: forall x e s, bstep' (x <- e) s (update x (e s) s)
 | s_seq: forall p q s s' s'', bstep' p s s' -> bstep' q s' s'' -> bstep' (p ;; q) s s''
-| s_ite_ff: forall e p q s s', teval e s = false -> bstep' q s s' -> bstep' (ite e p q) s s'
-| s_ite_tt: forall e p q s s', teval e s = true -> bstep' p s s' -> bstep' (ite e p q) s s'
-| s_whl_ff: forall e p s, teval e s = false -> bstep' (whl e p) s s
-| s_whl_tt: forall e p s s', teval e s = true -> bstep' (p ;; whl e p) s s' -> bstep' (whl e p) s s'.
+| s_ite_ff: forall (b: dset state) p q s s', b s = false -> bstep' q s s' -> bstep' (ite b p q) s s'
+| s_ite_tt: forall (b: dset state) p q s s', b s = true -> bstep' p s s' -> bstep' (ite b p q) s s'
+| s_whl_ff: forall (b: dset state) p s, b s = false -> bstep' (whl b p) s s
+| s_whl_tt: forall (b: dset state) p s s', b s = true -> bstep' (p ;; whl b p) s s' -> bstep' (whl b p) s s'.
 
 (** ** equivalence between the two definitions *)
 
@@ -167,10 +89,10 @@ Proof.
      eexists; eassumption. 
      right. eexists. split. reflexivity. simpl; now rewrite H. assumption.
      left. eexists. split. reflexivity. assumption. assumption. 
-     exists s. apply (str_refl ([e] * bstep p)). reflexivity.
+     exists s. apply (str_refl ([b] * bstep p)). reflexivity.
       simpl. unfold rel_inj. simpl. now rewrite H.
      destruct IHbstep' as [t ? [t' ? ?]]. exists t'. 2: assumption. 
-     apply (str_cons ([e] * bstep p)). exists t. 2: assumption.
+     apply (str_cons ([b] * bstep p)). exists t. 2: assumption.
      eexists; eauto. now split. 
   - induction p; unfold bstep; fold bstep.
      intros ? ? <-. constructor. 
@@ -192,7 +114,7 @@ Qed.
 Notation "p ~ q" := (bstep p == bstep q) (at level 80). 
 
 (** ad-hoc simplification tactic *)
-Ltac simp := unfold bstep; fold bstep; unfold teval; fold teval.
+Ltac simp := unfold bstep; fold bstep.
 
 
 (** ** denesting nested loops *)
@@ -213,171 +135,72 @@ Lemma dead_code b p q r:
 Proof. simp. kat. Qed.
 
 Lemma dead_code' a b p q r: 
-  (whl (a || b) p ;; ite b q r)  ~ 
-  (whl (a || b) p ;; r).
+  (whl (a \cup b) p ;; ite b q r)  ~ 
+  (whl (a \cup b) p ;; r).
 Proof. simp. kat. Qed.
 
 
 (** * Reasoning about assignations *)
 
-(** KAT cannot handle assignations: it's axioms mainly take care of
-   the control flow graph. We can however setup various tools to
-   reason about them manually. *)
+(** (higher-order style) substitution in formulas and expressions *)
+Definition subst x v (A: dset state): dset state := 
+  fun s => A (update x (v s) s).
+Definition esubst x v (e: state -> nat): state -> nat := 
+  fun s => e (update x (v s) s).
 
-(** ** free variables *)
+(** is [x] fresh in the expression e *)
+Definition fresh x (e: state -> nat) := forall v s, e (update x v s) = e s.
 
-Require Import lset.
-Notation " [[ p ]] " := (inj p): ra_terms. 
-
-Fixpoint fv e :=
-  match e with
-    | var x => [x]
-    | cst k => []
-    | pls e f 
-    | mul e f 
-    | min e f => fv e \cup fv f
-  end.
-
-Fixpoint tfv t :=
-  match t with
-    | tst e f => fv e \cup fv f
-    | cnj e f 
-    | dsj e f => tfv e \cup tfv f
-    | neg e => tfv e
-    | top 
-    | bot => []
-  end.
-
-(** ** substitutions *)
-
-Section s.
-Variable x: string. 
-Variable v: expr. 
-
-Fixpoint subst e: expr :=
-  match e with
-    | var y => if eqb x y then v else y
-    | cst k => k
-    | pls e f => subst e + subst f
-    | mul e f => subst e * subst f
-    | min e f => subst e - subst f
-  end%e.
-
-Fixpoint tsubst t: test :=
-  match t with
-    | tst e f => subst e ?= subst f
-    | cnj e f => tsubst e && tsubst f
-    | dsj e f => tsubst e || tsubst f
-    | neg e => neg (tsubst e)
-    | top => top
-    | bot => bot
-  end%t.
-
-(** ** bureaucratic lemmas about evalutaion and substitution *)
-
-Lemma eval_subst e s: eval (subst e) s = eval e (update x (eval v s) s).
-Proof. 
-  induction e; simpl; try congruence. 
-  unfold update; simpl. now case eqb_spec. 
-Qed.
-
-Lemma teval_subst t s: teval (tsubst t) s = teval t (update x (eval v s) s).
-Proof. 
-  induction t; simpl; try congruence. 
-  now rewrite 2eval_subst.
-Qed.
-
-Lemma subst_out e: ~In x (fv e) -> subst e = e.
-Proof.
-  induction e; simpl fv; simpl subst; rewrite ?in_app_iff; intros H.
-   case eqb_spec. 2: reflexivity. intros <-. elim H. now left. 
-   reflexivity. 
-   now rewrite IHe1, IHe2 by tauto.
-   now rewrite IHe1, IHe2 by tauto.
-   now rewrite IHe1, IHe2 by tauto.
-Qed.
-
-Lemma tsubst_out t: ~In x (tfv t) -> tsubst t = t.
-Proof.
-  induction t; simpl tfv; simpl tsubst; rewrite ?in_app_iff; intro H.
-   now rewrite 2subst_out by tauto. 
-   now rewrite IHt1, IHt2 by tauto.
-   now rewrite IHt1, IHt2 by tauto.
-   now rewrite IHt by assumption.
-   reflexivity. 
-   reflexivity.
-Qed.
-
-End s.
-
-Lemma eval_out x e: ~In x (fv e) -> forall i s, eval e (update x i s) = eval e s.
-Proof. intros. setoid_rewrite <-(eval_subst x i). now rewrite subst_out. Qed.
-
-Lemma teval_out x t: ~In x (tfv t) -> forall i s, teval t (update x i s) = teval t s.
-Proof. intros. setoid_rewrite <-(teval_subst x i). now rewrite tsubst_out. Qed.
-
-Lemma update_twice x i j s: update x j (update x i s) = update x j s.
-Proof. 
-  unfold update. apply functional_extensionality. intro y.
-  case eqb_spec; congruence. 
-Qed.
-
-Lemma update_comm x y i j s: x<>y -> update x i (update y j s) = update y j (update x i s).
-Proof. 
-  intro. unfold update. apply functional_extensionality. intro z.
-  case eqb_spec; case eqb_spec; congruence. 
-Qed.
+Hypothesis update_twice: forall x i j s, update x j (update x i s) = update x j s.
+Hypothesis update_comm: forall x y i j s, x<>y -> update x i (update y j s) = update y j (update x i s).
 
 
-(** ** back to program equivalences *)
+(** ** stacking assignations *)
 
-(** *** stacking assignations *)
 Lemma aff_stack x e f:
   (x <- e ;; x <- f)  ~  
-  (x <- subst x e f).
+  (x <- esubst x e f).
 Proof.
   simp. rewrite frel_comp.
   apply frel_weq; intro s. 
-  rewrite <-eval_subst. 
   apply update_twice.
 Qed.
 
-(** *** removing duplicates *)
-Lemma aff_idem x e: ~In x (fv e)  ->  
-  (x <- e ;; x <- e)  ~  (x <- e). 
+
+(** ** removing duplicates *)
+
+Lemma aff_idem x e: fresh x e -> (x <- e ;; x <- e)  ~  (x <- e). 
 Proof. 
   intro. rewrite aff_stack. 
-  now rewrite subst_out by assumption.
+  intros s s'. cbv. rewrite (H (e s)). tauto.
 Qed.
 
-(** *** commuting assignations *)
-Lemma aff_comm x y e f: x<>y  ->  
-  ~In y (fv e)  ->  
-  (x <- e ;; y <- f)  ~ (y <- subst x e f ;; x <- e).
+(** ** commuting assignations *)
+
+Lemma aff_comm x y e f: x<>y  -> fresh y e ->  
+  (x <- e ;; y <- f)  ~ (y <- esubst x e f ;; x <- e).
 Proof.
-  intros Hx Hy. simp. rewrite 2frel_comp. apply frel_weq; intro s. 
-  rewrite (eval_out y) by assumption.
-  rewrite eval_subst.
-  now rewrite update_comm by congruence.
+  intros Hx Hy. simp. rewrite 2frel_comp. apply frel_weq; intro s.
+  rewrite update_comm by congruence. 
+  now rewrite (Hy _). 
 Qed.
 
-(** *** delaying choices *)
+(** ** delaying choices *)
 
-(** in the above examples, we cannot exploit KAT since they are just
+(** in the above example, we cannot exploit KAT since this is just
    about assignations. In the following example, we show how to
-   perform a mixed proof: once we assert that the test [[t]] somehow
+   perform a mixed proof: once we assert that the test [t] somehow
    commutes with the assignation [x<-e], [hkat] can make use of this
    assumption to close the goal *)
 
 Lemma aff_ite x e t p q: 
   (x <- e ;; ite t p q)  
   ~ 
-  (ite (tsubst x e t) (x <- e ;; p) (x <- e ;; q)).
+  (ite (subst x e t) (x <- e ;; p) (x <- e ;; q)).
 Proof.
   simp. 
-  assert (H: upd x e * [[t]] == [[tsubst x e t]] * upd x e).
-   intros s s'. simpl. unfold rel_dot, rel_inj, frel. rewrite teval_subst. 
-   split. intros [? -> [<- ?] ]. eauto. intros [? [<- ?] ->]. eauto.
+  assert (H: upd x e * [t] == [subst x e t] * upd x e)
+   by (cbv; firstorder; subst; eauto). 
   hkat.
 Qed.
 
@@ -387,15 +210,15 @@ Qed.
 
 (** Hoare triples for partial correctness can be expressed really
    easily using KAT: *)
-Notation Hoare A p B := ([[teval A]] * bstep p * [[!teval B]] <== 0).
+Notation Hoare A p B := ([A] * bstep p * [!B] <== 0).
 
 (** ** correspondence w.r.t. the standard interpretation of Hoare triples  *)
 Lemma Hoare_eq A p B: 
   Hoare A p B <-> 
-  forall s s', teval A s -> bstep p s s' -> teval B s'.
+  forall s s', A s -> bstep p s s' -> B s'.
 Proof.
   split. 
-  - intros H s s' HA Hp. case_eq (teval B s'). reflexivity. intro HB. 
+  - intros H s s' HA Hp. case_eq (B s'). reflexivity. intro HB. 
     destruct (H s s'). exists s'. exists s. 
     now split. assumption. split. reflexivity. simpl. now rewrite HB. 
   - intros H s s' (?&?&<-&HA). intros Hp (->&HB). simpl in HB. 
@@ -418,18 +241,12 @@ Qed.
    The fact that we have an automatic tactic makes it trivial to
    formalise it. *)
 
-Lemma weakening (A A' B B': test) p: 
+Lemma weakening (A A' B B': dset state) p: 
   A' <== A -> Hoare A p B -> B <== B' -> Hoare A' p B'.
 Proof. hkat. Qed.
 
 Lemma rule_skp A: Hoare A skp A.
 Proof. simp. kat. Qed.
-
-Lemma rule_aff x v A: Hoare (tsubst x v A) (x <- v) A.
-Proof. 
-  rewrite Hoare_eq. intros s s' HA H. 
-  inversion_clear H. now rewrite <-teval_subst. 
-Qed.
 
 Lemma rule_seq A B C p q: 
   Hoare A p B -> 
@@ -438,23 +255,31 @@ Lemma rule_seq A B C p q:
 Proof. simp. hkat. Qed.
 
 Lemma rule_ite A B t p q: 
-  Hoare (A && t) p B -> 
-  Hoare (A && neg t) q B -> 
+  Hoare (A \cap t) p B -> 
+  Hoare (A \cap !t) q B -> 
   Hoare A (ite t p q) B.
 Proof. simp. hkat. Qed.
 
 Lemma rule_whl A t p: 
-  Hoare (A && t) p A -> 
-  Hoare A (whl t p) (A && neg t).
+  Hoare (A \cap t) p A -> 
+  Hoare A (whl t p) (A \cap neg t).
 Proof. simp. hkat. Qed.
 
+Lemma rule_aff x v (A: dset state): Hoare (subst x v A) (x <- v) A.
+Proof. 
+  rewrite Hoare_eq. intros s s' HA H. 
+  now inversion_clear H.
+Qed.
+
 Lemma wrong_rule_whl A t p: 
-  Hoare (A && neg t) p A -> 
-  Hoare A (whl t p) (A && neg t).
+  Hoare (A \cap !t) p A -> 
+  Hoare A (whl t p) (A \cap !t).
 Proof. simp. Fail hkat. Abort.
 
-Lemma rule_whl' (I A: test) t p: 
-  Hoare (I && t) p I -> 
-  teval (I && neg t) <== A -> 
+Lemma rule_whl' (I A: dset state) t p: 
+  Hoare (I \cap t) p I -> 
+  I \cap !t <== A -> 
   Hoare I (whl t p) A.
 Proof. eauto 3 using weakening, rule_whl. Qed.
+
+End s.
