paterson.v
@@ -1,0 +1,525 @@
+(*******************************************************************)
+(*  This is part of RelationAlgebra, it is distributed under the   *)
+(*    terms of the GNU Lesser General Public License version 3     *)
+(*              (see file LICENSE for more details)                *)
+(*                                                                 *)
+(*  Copyright 2013: Damien Pous. (CNRS, LIP - ENS Lyon, UMR 5668)  *)
+(*******************************************************************)
+
+
+(** * paterson: Equivalence of two flowchart schemes, due to Paterson
+   cf. "Mathematical theory of computation", Manna, 1974 
+   cf. "Kleene algebra with tests and program schematology", A. Angus and D. Kozen, 2001
+*)
+
+Require Import kat normalisation rewriting move kat_tac comparisons rel.
+Set Implicit Arguments.
+
+(** * Memory model  *)
+
+(** we need only five memory locations: the [y_i] are temporary
+   variables and [io] is used for input and output *)
+Inductive loc := y1 | y2 | y3 | y4 | io.
+Record state := { v1: nat; v2: nat; v3: nat; v4: nat; vio: nat }.
+
+(** getting the content of a memory cell *)
+Definition get x := match x with y1 => v1 | y2 => v2 | y3 => v3 | y4 => v4 | io => vio end.
+
+(** setting the content of a memory cell *)
+Definition set x n m := 
+  match x with
+    | y1 => {| v1:=n; v2:=v2 m; v3:=v3 m; v4:=v4 m; vio:=vio m |}
+    | y2 => {| v1:=v1 m; v2:=n; v3:=v3 m; v4:=v4 m; vio:=vio m |}
+    | y3 => {| v1:=v1 m; v2:=v2 m; v3:=n; v4:=v4 m; vio:=vio m |}
+    | y4 => {| v1:=v1 m; v2:=v2 m; v3:=v3 m; v4:=n; vio:=vio m |}
+    | io => {| v1:=v1 m; v2:=v2 m; v3:=v3 m; v4:=v4 m; vio:=n |}
+  end.
+
+(** basic properties of [get] and [set] *)
+Lemma get_set x v m: get x (set x v m) = v. 
+Proof. now destruct x. Qed.
+
+Lemma get_set' x y v m: x<>y -> get x (set y v m) = get x m. 
+Proof. destruct y; destruct x; simpl; trivial; congruence. Qed.
+
+Lemma set_set x v v' m: set x v (set x v' m) = set x v m.
+Proof. now destruct x. Qed.
+
+Lemma set_set' x y v v' m: x<>y -> set x v (set y v' m) = set y v' (set x v m).
+Proof. destruct y; destruct x; simpl; trivial; congruence. Qed.
+
+(** comparing locations *)
+Definition eqb x y :=
+  match x,y with
+    | y1,y1 | y2,y2 | y3,y3 | y4,y4 | io,io => true
+    | _,_ => false
+  end.
+Lemma eqb_spec: forall x y, reflect (x=y) (eqb x y).
+Proof. destruct x; destruct y; simpl; try constructor; congruence. Qed.
+Lemma eqb_false x y: x<>y -> eqb x y = false.
+Proof. case eqb_spec; congruence. Qed.
+Lemma neqb_spec x y: negb (eqb x y) <-> x<>y.
+Proof. case eqb_spec; intuition; congruence. Qed.
+
+
+(** * Arithmetic and Boolean expressions *)
+
+Section s.
+
+(** we assume arbitrary functions to interpret symbols [f], [g], and [p]  *)
+Variable ff: nat -> nat.
+Variable gg: nat -> nat -> nat. 
+Variable pp: nat -> bool. 
+
+(** we use a single inductive to represent Arithmetic and Boolean
+   expressions: this allows us to share code about evaluation, free
+   variables and so on, through polymorphism *)
+Inductive expr: Type -> Type :=
+  | e_var: loc -> expr nat
+  | O: expr nat
+  | f': expr nat -> expr nat
+  | g': expr nat -> expr nat -> expr nat
+  | p': expr nat -> expr bool
+  | e_cap: expr bool -> expr bool -> expr bool
+  | e_cup: expr bool -> expr bool -> expr bool
+  | e_neg: expr bool -> expr bool
+  | e_bot: expr bool
+  | e_top: expr bool.
+
+Coercion e_var: loc >-> expr.
+
+(** ** evaluation of expressions  *)
+Fixpoint eval A (e: expr A) (m: state): A :=
+  match e with
+    | e_var x => get x m
+    | O => 0%nat
+    | f' e => ff (eval e m)
+    | g' e f => gg (eval e m) (eval f m)
+    | p' e => pp (eval e m)
+    | e_cap e f => eval e m &&& eval f m
+    | e_cup e f => eval e m ||| eval f m
+    | e_neg e => negb (eval e m)
+    | e_bot => false
+    | e_top => true
+  end.
+
+
+(** ** Free variables *)
+
+Fixpoint free y A (e: expr A): bool :=
+  match e with
+    | e_var x => negb (eqb x y)
+    | f' e | p' e | e_neg e => free y e
+    | g' e f | e_cap e f | e_cup e f => free y e &&& free y f
+    | _ => true
+  end.
+
+(** ** Substitution *)
+
+Fixpoint subst x v A (f: expr A): expr A :=  
+  match f with
+    | e_var y => if eqb x y then v else e_var y
+    | O => O
+    | f' e => f' (subst x v e)
+    | p' e => p' (subst x v e)
+    | g' e f => g' (subst x v e) (subst x v f)
+    | e_cup e f => e_cup (subst x v e) (subst x v f)
+    | e_cap e f => e_cap (subst x v e) (subst x v f)
+    | e_neg e => e_neg (subst x v e)
+    | e_bot => e_bot
+    | e_top => e_top
+  end.
+
+Lemma subst_free x v A (e: expr A): free x e -> subst x v e = e.
+Proof.
+  induction e; simpl; trivial. 
+   rewrite neqb_spec. case eqb_spec; congruence.
+   intro. now rewrite IHe. 
+   rewrite landb_spec. intros [? ?]. now rewrite IHe1, IHe2. 
+   intro. now rewrite IHe. 
+   rewrite landb_spec. intros [? ?]. now rewrite IHe1, IHe2. 
+   rewrite landb_spec. intros [? ?]. now rewrite IHe1, IHe2. 
+   intro. now rewrite IHe. 
+Qed.
+
+Lemma free_subst x e A (f: expr A): free x e -> free x (subst x e f).
+Proof.
+  intro. induction f; simpl; rewrite ?IHf1; auto. 
+  case eqb_spec; trivial. simpl. rewrite neqb_spec. congruence.
+Qed.
+
+
+(** * Programs *)
+(** We just use KAT expressions, since any gflowchat scheme can be encoded as such an expression *)
+Inductive prog :=
+| p_tst(t: expr bool)
+| p_aff(x: loc)(e: expr nat)
+| p_str(p: prog)
+| p_dot(p q: prog)
+| p_pls(p q: prog).
+
+
+(** * Bigstep semantics *)
+
+(** updating the memory, according to the assignment [x<-e] *)
+Definition update x e m := set x (eval e m) m.
+(** relational counterpart of this function *)
+Notation upd x e := (frel (update x e)).
+
+(** Bigstep semantics, as a fixpoint *)
+Fixpoint bstep (p: prog): rel state state :=
+  match p with
+    | p_tst p => [eval p: dset state]
+    | p_aff x e => upd x e
+    | p_str p => bstep p ^*
+    | p_dot p q => bstep p * bstep q
+    | p_pls p q => bstep p + bstep q
+  end.
+
+(** auxiliary lemma relating the evaluation of expressions, the
+   assignments to the memory, and subsitution of expressions *)
+Lemma eval_update x v A (e: expr A) m: eval e (update x v m) = eval (subst x v e) m.
+Proof.
+  induction e; simpl; try congruence. 
+   unfold update. case eqb_spec. intros <-. apply get_set. 
+   intro. apply get_set'. congruence.
+  now rewrite IHe1, IHe2. 
+  now rewrite IHe1, IHe2. 
+Qed.
+
+
+(** Now we make the set of programs a Kleene algebra with tests: we
+   declare canonical structures for Boolean expressions (tests),
+   programs (Kleene elements), and the natural injection of the former
+   into the latter *)
+
+Canonical Structure expr_lattice_ops: lattice.ops := {|
+  car := expr bool;
+  leq := fun x y => eval x <== eval y;
+  weq := fun x y => eval x == eval y;
+  cup := e_cup;
+  cap := e_cap;
+  bot := e_bot;
+  top := e_top;
+  neg := e_neg
+|}.
+
+Canonical Structure prog_lattice_ops: lattice.ops := {|
+  car := prog;
+  leq := fun x y => bstep x <== bstep y;
+  weq := fun x y => bstep x == bstep y;
+  cup := p_pls;
+  cap := assert_false p_pls;
+  bot := p_tst e_bot;
+  top := assert_false (p_tst e_bot);
+  neg := assert_false id
+|}.
+
+Canonical Structure prog_monoid_ops: monoid.ops := {|
+  ob  := unit;
+  mor n m := prog_lattice_ops;
+  dot n m p := p_dot;
+  one n := p_tst e_top;
+  itr n := (fun x => p_dot x (p_str x));
+  str n := p_str;
+  cnv n m := assert_false id;
+  ldv n m p := assert_false (fun _ => id);
+  rdv n m p := assert_false (fun _ => id)
+|}.
+
+Canonical Structure prog_kat_ops: kat.ops := {|
+  kar := prog_monoid_ops;
+  tst n := expr_lattice_ops;
+  inj n := p_tst
+|}.
+
+Notation prog' := (prog_kat_ops tt tt).
+Notation test := (@tst prog_kat_ops tt).
+
+(** proving that the laws of KAT are satisfied is almost trivial,
+   since the model faithfully embeds in the relational model *)
+
+Instance expr_lattice_laws: lattice.laws BL expr_lattice_ops. 
+Proof.
+  apply laws_of_injective_morphism with (@eval bool: expr bool -> dset state); trivial. 
+  split; simpl; tauto.
+Qed.
+
+Instance prog_monoid_laws: monoid.laws BKA prog_monoid_ops. 
+Proof. 
+  apply laws_of_faithful_functor with (fun _ => state) (fun _ _: unit => bstep); trivial.
+  split; simpl; try discriminate; try tauto. 2: firstorder. 
+  split; simpl; try discriminate; try tauto. firstorder. 
+Qed.
+Instance prog_lattice_laws: lattice.laws BKA prog_lattice_ops := lattice_laws tt tt. 
+
+Instance prog_kat_laws: kat.laws prog_kat_ops. 
+Proof.
+  constructor; simpl; eauto with typeclass_instances. 2: tauto. 
+  split; try discriminate; try (simpl; tauto).
+  intros x y H. apply inj_leq. intro m. apply H.
+  intros x y H. apply inj_weq. intro m. apply H.
+  intros _ x y. apply (inj_cup (X:=rel_kat_ops)).
+  intros _ x y. apply (inj_cap (X:=rel_kat_ops)).
+Qed.
+
+(** ** variables read by a program *)
+
+(** [dont_read y p] holds if [p] never reads [y] *)
+Fixpoint dont_read y (p: prog'): bool :=
+  match p with
+    | p_str p => dont_read y p
+    | p_dot p q | p_pls p q => dont_read y p &&& dont_read y q
+    | p_aff x e => free y e
+    | p_tst t => free y t
+  end.
+
+
+
+(** ** Additional notation  *)
+
+Infix " ;" := (dot _ _ _) (left associativity, at level 40): ra_terms. 
+Definition aff x e: prog' := p_aff x e.
+Notation "x <- e" := (aff x e) (at level 30).
+Notation del y := (y<-O).
+
+
+(** * Laws of schematic KAT *)
+
+Opaque rel_monoid_ops rel_lattice_ops. 
+
+(** (the numbering corresponds to Angus and Kozen's paper)  *)
+Lemma eq_6 (x y: loc) (s t: expr nat): 
+  negb (eqb x y) &&& free y s -> x<-s;y<-t == y<-subst x s t; x<-s. 
+Proof.
+  rewrite landb_spec, neqb_spec. intros [D H]. simpl. 
+  rewrite 2frel_comp. apply frel_weq. intro m. 
+  unfold update at 1 2 3. rewrite set_set' by congruence. f_equal.  
+  now rewrite eval_update, subst_free.
+  unfold update. now rewrite <-eval_update.
+Qed.
+
+Lemma eq_7 (x y: loc) (s t: expr nat): 
+  negb (eqb x y) &&& free x s -> x<-s;y<-t == x<-s;y<-subst x s t. 
+Proof.
+  rewrite landb_spec, neqb_spec. intros [D H]. simpl. 
+  rewrite 2frel_comp. apply frel_weq. intro m. 
+  unfold update at 1 3. f_equal.  
+  rewrite 2eval_update. symmetry. rewrite subst_free. reflexivity. 
+  now apply free_subst.
+Qed.
+
+Lemma eq_8 (x: loc) (s t: expr nat): x<-s;x<-t == x<-subst x s t. 
+Proof.
+  simpl. rewrite frel_comp. apply frel_weq. intro m. 
+  unfold update. rewrite set_set. f_equal. apply eval_update. 
+Qed.
+
+Lemma eq_9 (x: loc) (t: expr nat) (phi: test): [subst x t phi: test];x<-t == x<-t;[phi].
+Proof.
+  Transparent rel_lattice_ops. intros m m'. split. Opaque rel_lattice_ops. 
+   intros [m0 [<- H] ->]. eexists. reflexivity. split; trivial. now rewrite eval_update.
+   intros [m0 -> [<- H]]. eexists. 2: reflexivity. split; trivial. now rewrite <-eval_update.
+Qed.
+
+
+Lemma eq_6' (x y: loc) (s t: expr nat): free x t &&& negb (eqb x y) &&& free y s -> 
+  x<-s;y<-t == y<-t; x<-s. 
+Proof. rewrite landb_spec. intros [? ?]. now rewrite eq_6, subst_free. Qed.
+
+Lemma eq_9' (x: loc) (t: expr nat) (phi: test): free x phi -> [phi];x<-t == x<-t;[phi].
+Proof. intro. now rewrite <-eq_9, subst_free. Qed.
+
+
+Lemma same_value (f: state -> state) (p: prog') (a b: test):
+  bstep p == frel f -> (forall m, eval a (f m) = eval b (f m)) -> 
+  p;[a\cap !b \cup !a\cap b] <== 0.
+Proof.
+  intros Hp H. simpl. rewrite Hp. 
+  Transparent rel_lattice_ops. intros m m' [? -> [<- E]]. Opaque rel_lattice_ops. 
+  exfalso. rewrite lorb_spec, 2landb_spec, 2negb_spec, H in E. intuition congruence.
+Qed.
+
+
+(** * Garbage-collecting assignments to unread variables *)
+
+(** (i.e., Lemma 4.5 in Angus and Kozen's paper)  *)
+Fixpoint gc y (p: prog'): prog' :=
+  match p with
+    | p_str p => gc y p^*
+    | p_tst _ => p
+    | p_aff x e => if eqb x y then 1 else x<-e
+    | p_dot p q => gc y p ; gc y q
+    | p_pls p q => gc y p + gc y q
+  end.
+
+Lemma gc_correct y p: dont_read y p -> gc y p; del y == p; del y.
+Proof.
+  Opaque prog_monoid_ops prog_lattice_ops prog_kat_ops.
+  intro H. transitivity (del y; gc y p).
+  induction p; simpl. 
+   now apply eq_9'.
+   case eqb_spec. ra. intro. apply eq_6'. now rewrite eqb_false. 
+   symmetry. apply str_move. symmetry. now auto. 
+   apply landb_spec in H as [? ?]. mrewrite IHp2. 2: assumption. now mrewrite IHp1.  
+   apply landb_spec in H as [? ?]. ra_normalise. now apply cup_weq; auto. 
+  symmetry. induction p; simpl. 
+   now apply eq_9'.
+   case eqb_spec. intros <-. rewrite eq_8. ra. intro D. apply eq_6'. now rewrite eqb_false. 
+   symmetry. apply str_move. symmetry. now auto. 
+   apply landb_spec in H as [? ?]. mrewrite IHp2. 2: assumption. now mrewrite IHp1.  
+   apply landb_spec in H as [? ?]. ra_normalise. now apply cup_weq; auto. 
+   Transparent prog_monoid_ops prog_lattice_ops prog_kat_ops.
+Qed.   
+
+
+(** * Paterson's equivalence *)
+Theorem Paterson: 
+  let a1 := p' y1: test in
+  let a2 := p' y2: test in
+  let a3 := p' y3: test in
+  let a4 := p' y4: test in
+  let clr := del y1; del y2; del y3; del y4 in
+  let x1 := y1<-io in
+  let s1 := y1<-f' io in
+  let s2 := y2<-f' io in
+  let z1 := io<-y1; clr in
+  let z2 := io<-y2; clr in
+  let p11 := y1<-f' y1 in
+  let p13 := y1<-f' y3 in
+  let p22 := y2<-f' y2 in
+  let p41 := y4<-f' y1 in
+  let q222 := y2<-g' y2 y2 in
+  let q214 := y2<-g' y1 y4 in
+  let q211 := y2<-g' y1 y1 in
+  let q311 := y3<-g' y1 y1 in
+  let r11 := y1<-f' (f' y1) in
+  let r12 := y1<-f' (f' y2) in
+  let r13 := y1<-f' (f' y3) in
+  let r22 := y2<-f' (f' y2) in
+  let rhs := s2;[a2];q222;([!a2];r22;[a2];q222)^*;[a2];z2 in
+  x1;p41;p11;q214;q311;([!a1];p11;q214;q311)^*;[a1];p13;
+  (([!a4]+[a4];([!a2];p22)^*;[a2\cap !a3];p41;p11);q214;q311;([!a1];p11;q214;q311)^*;[a1];p13)^*;
+  [a4];([!a2];p22)^*;[a2\cap a3];z2  ==  rhs.
+Proof.
+  intros.
+  (** simple commutation hypotheses, to be exploited by [hkat] *)
+  assert (a1p22:  [a1];p22  == p22;[a1])  by now apply eq_9'. 
+  assert (a1q214: [a1];q214 == q214;[a1]) by now apply eq_9'. 
+  assert (a1q211: [a1];q211 == q211;[a1]) by now apply eq_9'. 
+  assert (a1q311: [a1];q311 == q311;[a1]) by now apply eq_9'. 
+  assert (a2p13:  [a2];p13  == p13;[a2])  by now apply eq_9'. 
+  assert (a2r12:  [a2];r12  == r12;[a2])  by now apply eq_9'. 
+  assert (a2r13:  [a2];r13  == r13;[a2])  by now apply eq_9'. 
+  assert (a3p13:  [a3];p13  == p13;[a3])  by now apply eq_9'. 
+  assert (a3p22:  [a3];p22  == p22;[a3])  by now apply eq_9'. 
+  assert (a3r12:  [a3];r12  == r12;[a3])  by now apply eq_9'. 
+  assert (a3r13:  [a3];r13  == r13;[a3])  by now apply eq_9'. 
+  assert (a4p13:  [a4];p13  == p13;[a4])  by now apply eq_9'. 
+  assert (a4p11:  [a4];p11  == p11;[a4])  by now apply eq_9'. 
+  assert (a4p22:  [a4];p22  == p22;[a4])  by now apply eq_9'. 
+  assert (a4q214: [a4];q214 == q214;[a4]) by now apply eq_9'. 
+  assert (a4q211: [a4];q211 == q211;[a4]) by now apply eq_9'. 
+  assert (a4q311: [a4];q311 == q311;[a4]) by now apply eq_9'. 
+  assert (p41p11: p41;p11;[a1\cap !a4 \cup !a1\cap a4] <== 0).
+   eapply same_value. apply frel_comp. reflexivity. 
+  assert (q211q311: q211;q311;[a2\cap !a3 \cup !a2\cap a3] <== 0).
+   eapply same_value. apply frel_comp. reflexivity.
+  assert (r12p22: r12;p22;p22;[a1\cap !a2 \cup !a1\cap a2] <== 0).
+   eapply same_value. simpl. rewrite 2frel_comp. reflexivity. reflexivity.
+  (** this one cannot be used by [hkat], it's used by [rmov1]  *)
+  assert (p13p22: p13;p22 == p22;p13) by now apply eq_6'.
+
+  (** here starts the proof; the numbers in the comments refer to the
+     equation numbers in Angus and Kozen's paper proof *)
+
+  (** (19) *)
+  transitivity (
+    x1;p41;p11;q214;q311;
+    ([!a1\cap !a4];p11;q214;q311 +
+     [!a1\cap  a4];p11;q214;q311 +
+     [ a1\cap !a4];p13;[!a4];q214;q311 +
+     [a1\cap a4];p13;([!a2];p22)^*;[a2 \cap !a3];p41;p11;q214;q311)^*;
+    [a1];p13;([!a2];p22)^*;[a2 \cap a3 \cap a4];z2). 
+  clear -a4p13 a4p22. hkat. 
+  do 2 rmov1 p13.
+  (** (23+) *)
+  transitivity (
+    x1;p41;p11;q214;q311;
+    ([!a1\cap !a4];p11;q214;q311 +
+     [!a1\cap  a4];p11;q214;q311 +
+     [ a1\cap !a4];p13;[!a4];q214;q311 +
+     [a1\cap a4];p13;([!a2];p22)^*;[a2 \cap !a3];p41;p11;q214;q311)^*;
+    ([!a2];p22)^*;[a1 \cap a2 \cap a3 \cap a4];(p13;z2)). 
+  clear -a1p22; hkat. 
+  setoid_replace (p13;z2) with z2
+     by (unfold z2, clr; mrewrite <-(gc_correct y1); [ simpl; kat | reflexivity ]). 
+  (** (24) *)
+  transitivity (x1;p41;p11;q214;q311;
+    ([a1 \cap a4];p13;([!a2];p22)^*;[a2 \cap !a3];p41;p11;q214;q311)^*;
+    ([!a2];p22)^*;[a1 \cap a2 \cap a3 \cap a4];z2).
+  clear -p41p11 a1p22 a1q214 a1q311 a4p11 a4p13 a4p22 a4q214 a4q311; hkat.
+  (** big simplification w.r.t the paper proof here... *)
+
+  (** (27) *)
+  assert (p41p11q214: p41;p11;q214 == p41;p11;q211) by (simpl; now rewrite 3frel_comp).
+  do 2 mrewrite p41p11q214. clear p41p11q214.
+  (** (29) *)
+  transitivity (x1;(p41;(p11;q211;q311;[a1];p13;([!a2];p22)^*;[a2\cap!a3]))^*;
+                p41;p11;q211;q311;([!a2];p22)^*;[a1\cap a2\cap a3];z2).
+  clear -p41p11 a1p22 a1q211 a1q311 a4p22 a4q211 a4q311; hkat.
+  (** (31) *)
+  transitivity (x1;(p11;q211;q311;[a1];p13;([!a2];p22)^*;[a2\cap!a3])^*;
+                p11;q211;q311;([!a2];p22)^*;[a1\cap a2\cap a3];z2).
+  unfold z2, clr. mrewrite <-(gc_correct y4). 2: reflexivity. simpl. kat. 
+  (** (32) *)
+  rmov1 p13.
+  transitivity ((x1;p11);(q211;q311;([!a2];p22)^*;[a1\cap a2\cap!a3];(p13;p11))^*;
+                q211;q311;([!a2];p22)^*;[a1\cap a2\cap a3];z2).
+  clear -a1p22 a2p13 a3p13; hkat. 
+  (** big simplification w.r.t the paper proof here... *)
+
+  (** (33) *)
+  setoid_replace (x1;p11) with s1 by apply eq_8. 
+  setoid_replace (p13;p11) with r13 by apply eq_8. 
+  (** (34) *)
+  transitivity (s1;(q211;q311;(([!a2];p22)^*;([a1];r13));[a2\cap!a3])^*;
+                q211;q311;([!a2];p22)^*;[a1\cap a2\cap a3];z2).
+  clear -a2r13 a3r13; hkat. 
+  setoid_replace (([!a2];p22)^*;([a1];r13)) with ([a1];r13;([!a2];p22)^*)
+   by (assert (r13;p22 == p22;r13) by (now apply eq_6'); rmov1 r13; clear -a1p22; hkat). 
+  transitivity (s1;([a1];(q211;q311;r13);([!a2];p22)^*;[a2\cap!a3])^*;
+                q211;q311;([!a2];p22)^*;[a1\cap a2\cap a3];z2).
+  clear -a1q311 a1q211; hkat. 
+  (** (35) *)
+  setoid_replace (q211;q311;r13) with (q211;q311;r12) by (simpl; now rewrite 3frel_comp).
+  (** (36) *)
+  transitivity (s1;([a1];(q211;q311);[!a2];r12;([!a2];p22)^*;[a2])^*;
+                (q211;q311);[a2];([!a2];p22)^*;[a1\cap a2];z2).
+  clear -a3p22 a3r12 q211q311. hkat. 
+  (** (37) *)
+  transitivity (s1;([a1];q211;[!a2];r12;([!a2];p22)^*;[a2])^*;
+                q211;[a2];([!a2];p22)^*;[a1\cap a2];z2).
+  unfold z2, clr. mrewrite <-(gc_correct y3). 2: reflexivity. simpl. kat. 
+  (** (38) *)
+  transitivity (s1;[a1];q211;([!a2];r12;[a1];p22;[a2];q211 + 
+                              [!a2];r12;[a1];p22;[!a2];(p22;q211))^*;[a2];z2).
+  clear -a1p22 a1q211 a2r12 r12p22 a1p22. hkat. 
+  (** big simplification w.r.t the paper proof here... *)
+
+  (** (43) *)
+  assert (p22q211: p22;q211 == q211) by apply eq_8. rewrite p22q211.
+  transitivity (s1;[a1];q211;([!a2];r12;[a1];(p22;q211))^*;[a2];z2). kat.
+  rewrite p22q211. clear p22q211.
+  (** (44) *)
+  unfold s1, a1, q211, r12, a2. rewrite <-eq_9. mrewrite eq_7. 2: reflexivity.
+  mrewrite <-eq_9. mrewrite (eq_7 y1 y2 (f' (f' y2))). 2: reflexivity.
+  unfold z2, clr. mrewrite <-(gc_correct y1). 2: reflexivity.
+  unfold rhs, z2, clr, s2, a2. rewrite <-eq_9.
+  unfold q222. mrewrite eq_7. 2: reflexivity.
+  unfold r22. mrewrite <-eq_9. do 2 mrewrite eq_8.
+  simpl gc. kat. 
+  (** (47) *)
+Qed.
+
+End s.
